Sketch code to use cProp for elaboration

WIP/CompProp.v
@@ -10,6 +10,8 @@ Open Scope list.
 Require Import Utils.Base Utils.Booleans Utils.Eqb.
 *)
 Require Import Utils (*TODO: temp*).
+Require Import Utils.Monad.
+Import StateMonad.
 
 (* Not definitions so that they don't get in the way of evaluation
  *)
@@ -57,6 +59,20 @@ Proof. solve_corresponds. Qed.
 #[export] Instance cfalse_corresponds : cCorresponds cFalse (fun _ => False).
 Proof. solve_corresponds. Qed.
 
+Ltac inhabited_corresponds v :=
+  unfold cCorresponds in *;
+    cbn;
+    intuition idtac;
+  constructor; eauto;
+  apply v.
+
+
+#[export] Instance inhabited_Prop_corresponds : cCorresponds cTrue (fun t => inhabited Prop).
+Proof. inhabited_corresponds True. Qed.
+
+(*TODO: always use this one or defer to ones like above sometimes? *)
+#[export] Instance inhabited_default_corresponds X `{WithDefault X} : cCorresponds cTrue (fun _ => inhabited X).
+Proof. inhabited_corresponds default. Qed.
 
 Definition cand (a b : cProp) :=
   match a, b with
@@ -107,15 +123,6 @@ Definition ciff (a b : cProp) :=
   | cEmbed P1, cEmbed P2 => cEmbed (lift2 iff P1 P2)
   end.
 
-
-#[export] Instance Prop_corresponds : cCorresponds cTrue (fun t => inhabited Prop).
-Proof.  
-  unfold cCorresponds in *;
-    cbn;
-    intuition idtac.
-  constructor; eauto.
-  apply True.
-Qed.
 
 Section WithParams.
   Context (cB' cB : cProp) (B' B : forall x : A, (*E x ->*) Prop)
@@ -242,14 +249,15 @@ Admitted.
 
 
 Definition cexists T A (cA : cProp T) (cP : cProp {t : T & A t}) : cProp T :=
-  match cP with
-  | cTrue _ => cA
-  (* must check the inhabitance of A
-     Question: should I design this to assume A inhabited?
-   *)
-  | cFalse _ => cFalse _
-  | cEmbed P => cEmbed (fun t => exists x : A t, P (existT _ t x))
+  match cA, cP with
+  | _, cFalse _
+  | cFalse _, _ => cFalse _
+  | cTrue _, cTrue _ => cTrue _
+  | cEmbed P, cTrue _ => cEmbed P
+  | cTrue _, cEmbed P
+  | cEmbed _, cEmbed P =>  cEmbed (fun t => exists x : A t, P (existT _ t x))
   end.
+    
 (*
 #[export] Instance cexist_corresponds T A cB (B : forall t : T, A t -> Prop)
   `{cCorresponds (sigT A)%type cB (fun t' => B (projT1 t') (projT2 t'))}
@@ -300,11 +308,334 @@ Proof.
 Qed.
 
 
+Ltac solve_corresponds :=
+  unfold cCorresponds in*;
+  repeat lazymatch goal with [P : cProp _ |- _] => destruct P;try clear P end;
+  cbn in *; intros a;
+  repeat match goal with [H : forall a (* (e : E a)*), _ |- _] => specialize (H a) end;
+  intuition fail.
 
-Definition cIs_true (b : bool) := if b then cTrue else cFalse.
 
-#[export] Instance cIstrue_corresponds b : cCorresponds (cIs_true b) (Is_true b).
+Definition cIs_true {T} (b : bool) : cProp T := if b then cTrue _ else cFalse _.
+
+#[export] Instance cIstrue_corresponds T b : cCorresponds (cIs_true b) (fun t : T=> Is_true b).
 Proof. destruct b; solve_corresponds. Qed.
+
+
+
+Fixpoint call2 {T A B} (R : A -> B -> cProp T) l1 l2 : cProp T :=
+  match l1, l2 with
+  | [], [] => cTrue _
+  | a::l1, b::l2 => cand (R a b) (call2 R l1 l2)
+  | _, _ => cFalse _
+  end.
+
+
+Instance call2_corresponds {T A B} cR (R : T -> A -> B -> Prop)
+  `{forall a b, cCorresponds (cR a b) (fun t => R t a b)}
+  l1 l2
+  : cCorresponds (call2 cR l1 l2) (fun t:T => Forall2 (R t) l1 l2).
+Proof.
+  revert l2;
+    induction l1; destruct l2; basic_goal_prep.
+  1-3:cbv; intuition eauto; safe_invert H0.
+  {
+    assert (forall t, Forall2 (R t) (a :: l1) (b :: l2) <-> R t a b /\ Forall2 (R t) l1 l2).
+    {
+      intuition eauto;safe_invert H0; tauto.
+    }
+    unfold cCorresponds.
+    intro t.
+    rewrite H0.
+    revert t.
+    change (cCorresponds (cand (cR a b) (call2 cR l1 l2)) (fun t => R t a b /\ Forall2 (R t) l1 l2)).
+    typeclasses eauto.
+  }
+Qed.
+
+Require Import Pyrosome.Theory.Core Pyrosome.Elab.Elab.
+
+
+Section WithVar.
+  Context (V : Type)
+    {V_Eqb : Eqb V}
+    {V_Eqb_ok : Eqb_ok V_Eqb}
+          {V_default : WithDefault V}.
+
+  Notation named_list := (@named_list V).
+  Notation named_map := (@named_map V).
+  Notation term := (@term V).
+  Notation ctx := (@ctx V).
+  Notation sort := (@sort V).
+  Notation subst := (@subst V).
+  Notation rule := (@rule V).
+  Notation lang := (@lang V).
+
+   Section WithLang.
+
+     Context (l : lang).
+
+     Section WithCtx.
+    Context (c : ctx).
+
+    Section Inner.
+      Context (celab_term : term -> term -> sort -> cProp unit).
+      Fixpoint celab_args s args es c' {struct es} : cProp unit :=
+        match c', es, args, s with
+        | [], [], [], [] => cTrue _
+        | _, _, _::_, []
+        | _, _, [],  _::_
+        | [], _, _::_, _
+        | [], _::_, _, _
+        | _::_, [], _, _ => cFalse _
+        | (name,t')::c'', ee::es', [], [] =>
+            cand (cEmbed (fun _ => wf_term l c ee t'[/with_names_from c'' es'/]))
+                 (celab_args [] [] es' c'')
+        | (name,t')::c'', ee::es', name'::args', e::s' =>
+            if eqb name name'
+            then
+              cand (celab_term e ee t'[/with_names_from c'' es'/])
+                (celab_args s' args' es' c'')
+            else
+              cand (cEmbed (fun _ => wf_term l c ee t'[/with_names_from c'' es'/]))
+                (celab_args s args es' c'')
+        end.
+    End Inner.
+
+    Fixpoint celab_term (e ee : term) t : cProp unit :=
+      match e, ee with
+      | var x, var ex =>
+          cIs_true (andb (eqb x ex)
+                      (eqb (named_list_lookup_err c x) (Some t)))
+      | con name s, con ename es =>
+          cand (cIs_true (eqb name ename))
+          match named_list_lookup_err l name with
+          | Some (term_rule c' args t') =>
+              (*TODO: use eq_term variant w/ full refl (TODO: finish that one's proof) *)
+              (cand (cEmbed (fun _ => eq_sort l c t t'[/with_names_from c' es/]))
+                 (celab_args celab_term s args es c'))
+          | _ => cFalse _
+          end
+      | _, _ => cFalse _
+      end.
+
+    Definition celab_sort (t et : sort) : cProp unit :=
+      let (name, s) := t in
+      let (ename, es) := et in
+      cand (cIs_true (eqb name ename))
+        match named_list_lookup_err l name with
+        | Some (sort_rule c' args) =>
+            (celab_args celab_term s args es c')
+        | _ => cFalse _
+        end.
+
+    Section __.
+      Context (evars : nat -> term).
+      (*TODO: generalizes Utils.Gensym; move there*)
+      Definition fresh {M} `{Monad M} : stateT nat M nat :=
+        fun n => Mret (n, S n).
+
+      Section Inner.
+        Context (gen_elab_term : term -> stateT nat option term).
+
+        Definition gen_elab_args_body gen_elab_args1 gen_elab_args2
+          s args (c' : ctx) : stateT nat option (list term) :=
+          match c', args, s with
+          | [], [], [] => @! ret []
+          | _, _::_, []
+          | _, [], _::_
+          | [], _, _ => fun _ : nat => None
+          | (n,_)::c'', [], [] =>
+              @!let s_out <- gen_elab_args1 c'' in
+                let x <- fresh (M:=option) in                
+                let ee : term := evars x in
+                ret (ee::s_out)
+          | (n,_)::c'', n'::args', e::s' =>
+              if eqb n n'
+              then @!let s_out <- gen_elab_args2 s' args' c'' in
+                     let ee <- gen_elab_term e in
+                     ret (ee::s_out)
+              else @!let s_out <- gen_elab_args1 c'' in
+                     let x <- fresh (M:=option) in                
+                     let ee := evars x in
+                     ret (ee::s_out)
+          end.
+
+        Section InnerInner.
+          
+        Context (gen_elab_args : list term -> list V -> list (V * sort) -> stateT nat option (list term)).
+        Context (s : list term) (args : list V).
+        Fixpoint gen_elab_args1 (c' : ctx) {struct c'} : stateT nat option (list term) :=
+          gen_elab_args_body gen_elab_args1 gen_elab_args s args c'.
+
+        End InnerInner.
+                             
+        Fixpoint gen_elab_args s args (c' : ctx) {struct s} : stateT nat option (list term) :=
+          gen_elab_args_body (gen_elab_args1 gen_elab_args s args) gen_elab_args s args c'.
+
+      End Inner.
+
+      Fixpoint gen_elab_term (e : term) :  stateT nat option term :=
+        match e with
+        | var x => Mret (var x)
+        | con n s =>
+          match named_list_lookup_err l n with
+          | Some (term_rule c' args t') =>
+              @!let s' <- gen_elab_args gen_elab_term s args c' in
+                ret (con n s')
+          | _ => fun _ : nat => None
+          end
+        end.
+
+      
+      Definition gen_elab_sort (t : sort) :  stateT nat option sort :=
+        match t with
+        | scon n s =>
+          match named_list_lookup_err l n with
+          | Some (sort_rule c' args) =>
+              @!let s' <- gen_elab_args gen_elab_term s args c' in
+                ret (scon n s')
+          | _ => fun _ : nat => None
+          end
+        end.
+
+      (*Definition gen_elab_term (e : term) : option term :=
+        option_map fst (gen_elab_term' e 0).*)
+
+    End __.
+
+     End WithCtx.
+
+     
+     Fixpoint celab_ctx (c ec : ctx) :=
+       match c, ec with
+       | [], [] => cTrue _
+       | (n,t)::c', (en,et)::ec' =>
+           cand (cIs_true (eqb n en))
+             (cand (celab_ctx c' ec')
+                (celab_sort ec' t et))                  
+       | _, _ => cFalse _
+       end.
+     
+     (* TODO: check that evars from ectx ending up in eqbs isn't a problem
+        (should probably end up in eq_sort, but worth checking)
+      *)
+    Definition celab_rule (r er : rule) : cProp unit :=
+      match r, er with
+      | sort_rule c args, sort_rule ec eargs =>
+          cand (cIs_true (eqb args eargs))
+               (celab_ctx c ec)
+      | term_rule c args t, term_rule ec eargs et =>
+          cand (cIs_true (eqb args eargs))
+               (cand (celab_sort ec t et)
+                  (celab_ctx c ec))
+      | sort_eq_rule c t t', sort_eq_rule ec et et'=>
+          cand (celab_sort ec t et)
+            (cand (celab_sort ec t' et')
+               (celab_ctx c ec))
+      | term_eq_rule c e e' t, term_eq_rule ec ee ee' et =>
+          cand (celab_sort ec t et)
+            (cand (celab_term ec e ee et)
+               (cand (celab_term ec e' ee' et)
+                  (celab_ctx c ec)))
+      | _, _ => cFalse _
+      end.
+
+    Section __.
+      Context (evars : nat -> term).
+
+      
+     Definition gen_elab_ctx : ctx -> stateT nat option ctx :=
+       list_Mmap
+         (fun '(n,t) =>
+            @!let t' <- gen_elab_sort evars t in
+              ret (n,t')).
+   
+    
+    Definition gen_elab_rule r : stateT nat option rule :=
+      match r with
+      | sort_rule c args =>
+          @! let ec <- gen_elab_ctx c in
+             ret sort_rule ec args
+      | term_rule c args t =>
+          @! let ec <- gen_elab_ctx c in
+             let et <- gen_elab_sort evars t in
+             ret term_rule ec args et
+      | sort_eq_rule c t t'=>
+          @! let ec <- gen_elab_ctx c in
+             let et <- gen_elab_sort evars t in
+             let et' <- gen_elab_sort evars t' in
+             ret sort_eq_rule ec et et'
+      | term_eq_rule c e e' t =>
+          @! let ec <- gen_elab_ctx c in
+             let et <- gen_elab_sort evars t in
+             let ee <- gen_elab_term evars e in
+             let ee' <- gen_elab_term evars e' in
+             ret term_eq_rule ec ee ee' et
+      end.
+
+    End __.
+    
+   End WithLang.
+
+   
+     Fixpoint celab_lang (l el : lang) :=
+       match l, el with
+       | [], [] => cTrue _
+       | (n,r)::l', (en,er)::el' =>
+           cand (cIs_true (eqb n en))
+             (cand (celab_lang l' el')
+                (celab_rule el' r er))                  
+       | _, _ => cFalse _
+       end.
+      
+     Fixpoint gen_elab_lang evars (l : lang) : stateT nat option lang :=
+       match l with
+       | [] => Mret []
+       | (n,r)::l' =>
+           @!let el' <- gen_elab_lang evars l' in
+             let r' <- gen_elab_rule el' evars r in
+             ret {(stateT nat option)} (n,r')::el'
+       end.
+                                              
+        
+
+   End WithVar.
+      
+Require Import String List Pyrosome.Lang.SimpleVSubst
+  Pyrosome.Lang.SimpleVSTLC.
+Import Core.Notations ListNotations.
+
+Goal False.
+  epose (gen_elab_lang _ SimpleVSubst.value_subst_def 0) as vs.
+  vm_compute in vs.
+  let v := eval cbv in vs in
+  match v with
+  | Some ?vs' => clear vs; pose vs' as vs
+  end.
+  let l' := eval compute in value_subst in
+  assert (interp tt (celab_lang (skipn 19 l') (skipn 19 (fst vs)))).
+  {
+    cbn [skipn fst vs].
+    TODO: issue on first eqn
+    vm_compute.
+    cbn [celab_lang fst vs celab_rule celab_ctx celab_sort celab_term].
+    cbn.
+  Compute PolySubst.val_subst.
+  epose (gen_elab_ctx value_subst _ [("G", {{s #"env" }})] 0) as c.
+  cbn in c.
+  epose (gen_elab_sort value_subst _  {{s #"env" }} 0) as t.
+  cbn in t.
+  TODO: ctx issues?
+  TODO: why None?
+  epose ((gen_elab_term (stlc++(SimpleVSubst.exp_subst ++ SimpleVSubst.value_subst)%list)
+            _ {{e #"lambda" "A" #"hd" }}) 0).
+  cbn in o.
+  unfold Basics.compose, uncurry in s.
+Eval cbn in .
+      
+
+
 
 Section WithDecidable.
 
@@ -341,34 +672,6 @@ Proof.
   induction l; basic_goal_prep; typeclasses eauto.
 Qed.
 
-
-Fixpoint call2 {A B} (R : A -> B -> cProp) l1 l2 : cProp :=
-  match l1, l2 with
-  | [], [] => cTrue
-  | a::l1, b::l2 => cand (R a b) (call2 R l1 l2)
-  | _, _ => cFalse
-  end.
-
-
-Instance call2_corresponds {A B} cR (R : A -> B -> Prop)
-  `{forall a b, cCorresponds (cR a b) (R a b)}
-  l1 l2
-  : cCorresponds (call2 cR l1 l2) (Forall2 R l1 l2).
-Proof.
-  revert l2;
-    induction l1; destruct l2; basic_goal_prep.
-  1-3:cbv; intuition eauto; safe_invert H0.
-  {
-    assert (Forall2 R (a :: l1) (b :: l2) <-> R a b /\ Forall2 R l1 l2).
-    {
-      intuition eauto;safe_invert H0; tauto.
-    }
-    unfold cCorresponds.
-    rewrite H0.
-    change (cCorresponds (cand (cR a b) (call2 cR l1 l2)) (R a b /\ Forall2 R l1 l2)).
-    typeclasses eauto.
-  }
-Qed.
 
 
 
